src/TypesExt.v
@@ -15,8 +15,24 @@ Class Iso (A B : Type) : Type :=
 ; outof : B -> A
 }.
 
+Class StrongIso (A B : Type) : Type :=
+{ sinto : forall (P : Type -> Type), P A -> P B
+; soutof : forall (P : Type -> Type), P B -> P A
+}.
+
+Class StrongIsoOk A B (SIso : StrongIso A B) : Type :=
+{ into_outof : forall R x,
+  sinto R (soutof R x) = x
+; outof_into : forall R x,
+  soutof R (sinto R x) = x
+}.
+
+Arguments sinto {_ _} {iso} P _ : rename.
+Arguments soutof {_ _} {iso} P _ : rename.
+
 Class RType (typ : Type) (typD : list Type -> typ -> Type) : Type :=
-{ typ_cast : forall env (a b : typ), option (typD env a -> typD env b)
+{ typ_cast : forall (F : Type -> Type) env (a b : typ), option (F (typD env a) -> F (typD env b))
+; typ_eqb : typ -> typ -> bool
 ; eqb : forall ts (t : typ), (forall a b : typD ts t, option bool)
 ; typeFor : forall ts (t : typ), type (typD ts t)
 ; instantiate_typ : list typ -> typ -> typ
@@ -27,24 +43,33 @@ Class RType (typ : Type) (typD : list Type -> typ -> Type) : Type :=
 }.
 
 Class RTypeOk typ typD (RType_typ : @RType typ typD) : Type :=
-{ eqb_ok : forall ts t a b,
+{ (** eqb **)
+  eqb_ok : forall ts t a b,
              match eqb ts t a b with
                | None => True
                | Some true => equal (type := typeFor _ t) a b
                | Some false => ~equal (type := typeFor _ t) a b
              end
-; typ_cast_iso : forall ts a b f, 
-    typ_cast ts a b = Some f ->
+  (** typ_eqb **)
+; typ_eqb_ok : forall a b, typ_eqb a b = true -> a = b
+  (** typ_cast **)
+; typ_cast_iso : forall F ts a b f, 
+    typ_cast F ts a b = Some f ->
     exists g, 
-      typ_cast ts b a = Some g /\
+      typ_cast F ts b a = Some g /\
       (forall x, f (g x) = x)
-; typ_cast_refl : forall ts t, 
-                    exists f, typ_cast ts t t = Some f /\
+; typ_cast_refl : forall ts t F, 
+                    exists f, typ_cast F ts t t = Some f /\
                               (forall x, f x = x)
+  (** type_of_apply **)
 ; type_of_apply_nil : forall t, type_of_apply t nil = Some t
-; type_of_apply_cons : forall t t' t'' ts, 
-  type_of_apply t (Some t' :: ts) = Some t'' <-> 
-  
+; type_of_apply_cons : forall t t' t'' ts ts', 
+  type_of_apply t (Some t' :: ts) = Some t'' ->
+  exists T, typD ts' t = (typD ts' t' -> typD ts' T) /\
+            type_of_apply T ts = Some t''  
+; type_of_apply_None_cons : forall t ts, 
+  type_of_apply t (None :: ts) = None
+  (** instantiate_typ **)
 }.
 
 Section typed.
@@ -70,32 +95,99 @@ Section typed.
 *)
 
   Class TypInstance0 (F : Type) : Type :=
-  { ctor0     : typ
-  ; ctor0_iso : forall ts, Iso F (typD ts ctor0)
-  ; ctor0_match : forall ts (R : typ -> Type -> Type)
-      (caseCtor : unit -> R ctor0 F)
+  { typ0     : typ
+  ; typ0_iso : forall ts, StrongIso F (typD ts typ0)
+  ; typ0_match : forall ts (R : typ -> Type -> Type)
+      (caseTyp : unit -> R typ0 F)
       (caseElse : forall t : typ, R t (typD ts t))
       (t : typ), R t (typD ts t)
+  }.
+
+  Class TypInstance0_Ok F (ti : TypInstance0 F) : Type :=
+  { typ0_match_typ0 : forall ts R caseTyp caseElse,
+      (typ0_match ts R caseTyp caseElse typ0) = sinto (iso := typ0_iso ts) _ (caseTyp tt)
+  ; typ0_isoOk : forall ts, StrongIsoOk (typ0_iso ts)
   }.
 
   Class TypInstance1 (F : Type -> Type) : Type :=
-  { ctor1     : typ -> typ
-  ; ctor1_iso : forall ts t, Iso (F (typD ts t)) (typD ts (ctor1 t))
-  ; ctor1_match : forall ts (R : typ -> Type -> Type)
-      (caseCtor : forall t, R (ctor1 t) (typD ts (ctor1 t)))
+  { typ1     : typ -> typ
+  ; typ1_iso : forall ts t,
+                  StrongIso (F (typD ts t)) (typD ts (typ1 t))
+  ; typ1_match : forall ts (R : typ -> Type -> Type)
+      (caseTyp : forall t, R (typ1 t) (F (typD ts  t)))
       (caseElse : forall t : typ, R t (typD ts t))
       (t : typ), R t (typD ts t)
+  }.
+
+  Class TypInstance1_Ok F (ti : TypInstance1 F) : Type :=
+  { typ0_match_typ1 : forall ts R caseTyp caseElse t,
+      (typ1_match ts R caseTyp caseElse (typ1 t)) = sinto (iso := typ1_iso ts t) _ (caseTyp t)
+  ; typ1_isoOk : forall ts t, StrongIsoOk (typ1_iso ts t)
   }.
 
   Class TypInstance2 (F : Type -> Type -> Type) : Type :=
-  { ctor2     : typ -> typ -> typ
-  ; ctor2_iso : forall ts t1 t2, Iso (F (typD ts t1) (typD ts t2)) (typD ts (ctor2 t1 t2))
-  ; ctor2_match : forall ts (R : typ -> Type -> Type)
-      (caseCtor : forall t1 t2, R (ctor2 t1 t2) (typD ts (ctor2 t1 t2)))
+  { typ2     : typ -> typ -> typ
+  ; typ2_iso : forall ts t1 t2, 
+                  StrongIso (F (typD ts t1) (typD ts t2)) (typD ts (typ2 t1 t2))
+  ; typ2_match : forall ts (R : typ -> Type -> Type)
+      (caseTyp : forall t1 t2, R (typ2 t1 t2) (F (typD ts t1) (typD ts t2)))
       (caseElse : forall t : typ, R t (typD ts t))
       (t : typ), R t (typD ts t)
   }.
 
+  Class TypInstance2_Ok F (ti : TypInstance2 F) : Type :=
+  { typ2_match_typ1 : forall ts R caseTyp caseElse t u,
+      (typ2_match ts R caseTyp caseElse (typ2 t u)) = sinto (iso := typ2_iso ts t u) _ (caseTyp t u)
+  ; typ2_isoOk : forall ts t u, StrongIsoOk (typ2_iso ts t u)
+  }.
+
+  Section instances.
+    Global Instance TypInstance0_app F T 
+           (f : TypInstance1 F) (t : TypInstance0 T)
+    : TypInstance0 (F T) :=
+    { typ0 := typ1 typ0
+    ; typ0_iso := fun ts => {| sinto := fun _ => _ ; soutof := fun _ => _ |}
+    ; typ0_match := fun ts R caseTyp caseElse t =>
+        typ1_match ts R (fun t' => 
+                           typ0_match ts (fun ty Ty => R (typ1 ty) (F Ty)) 
+                                      caseTyp
+                                      (fun _ => _) t') caseElse t 
+    }.
+    { apply typ1_iso. apply typ0_iso. refine (fun x => x). }
+    { apply typ1_iso. apply typ0_iso. refine (fun x => x). }
+    { apply typ1_iso. apply caseElse. }
+    Defined.
+
+    Global Instance TypInstance0_app2 F T1 T2 
+           (f : TypInstance2 F) (t1 : TypInstance0 T1) (t2 : TypInstance0 T2) 
+    : TypInstance0 (F T1 T2) :=
+    { typ0 := typ2 (typ0 (TypInstance0 := t1)) (typ0 (TypInstance0 := t2))
+    ; typ0_iso := fun ts => {| sinto := fun _ => _ ; soutof := fun _ => _ |}
+    ; typ0_match := fun ts R caseTyp caseElse t =>
+        typ2_match ts R 
+           (fun t1' t2' => 
+              typ0_match (TypInstance0 := t1) ts 
+                 (fun ty Ty => R (typ2 ty t2') (F Ty (typD ts t2')))
+                 (fun _ =>
+                    typ0_match (TypInstance0 := t2) ts
+                        (fun ty Ty => R (typ2 (typ0 (TypInstance0 := t1)) ty)
+                                        (F T1 Ty))
+                        caseTyp
+                        (fun _ => _)
+                        t2')
+                 (fun _ => _)
+                 t1') caseElse t
+
+    }.
+    { apply typ2_iso. apply typ0_iso. apply typ0_iso. refine (fun x => x). }
+    { apply typ2_iso. apply typ0_iso. apply typ0_iso. refine (fun x => x). }
+    { eapply (soutof (iso := typ0_iso ts) (fun x => R (typ2 typ0 t0) (F x (typD ts t0)))). 
+      eapply (soutof (iso := typ2_iso ts _ _) _).
+      apply caseElse. }
+    { eapply (soutof (iso := typ2_iso ts _ _) _). 
+      apply caseElse. }
+    Defined.
+
+  End instances.
 
 End typed.  
-
