src/ExprExtDemo.v
@@ -1,0 +1,157 @@
+Require Import List Bool.
+Require Import ExtLib.Data.Fun.
+Require Import ExtLib.Data.HList.
+Require Import ExtLib.Structures.Monad.
+Require Import MirrorCore.TypesExt.
+Require Import MirrorCore.ExprExt.
+
+Set Implicit Arguments.
+Set Strict Implicit.
+
+Section Demo.
+
+  Variable m : Type -> Type.
+  Context {Monad_m : Monad m}.
+
+  Variable typ : Type.
+  Variable typD : list Type -> typ -> Type.
+  Context {RType_typ : RType typD}.
+  Context {RTypeOk_typ : RTypeOk RType_typ}.
+  Context {typ_arr : TypInstance2 typD Fun}.
+  Context {typ_m : TypInstance1 typD m}.
+  Context {typ_nat : TypInstance0 typD nat}.
+  Let tvNat := @typ0 _ typD _ typ_nat.
+  Let nat_match := @typ0_match _ typD _ typ_nat.
+  Let nat_into (F : Type -> Type) ts : F nat -> F (typD ts tvNat) :=
+    into (Iso := @typ0_iso _ _ _ typ_nat F ts).
+  Let tvArr := @typ2 _ typD _ typ_arr.
+  Let arr_match := @typ2_match _ typD _ typ_arr.
+  Let arr_into (F : Type -> Type) ts a b : F (typD ts a -> typD ts b) -> F (typD ts (tvArr a b)) :=
+    into (Iso := @typ2_iso _ _ _ typ_arr F ts a b).
+  Let arr_outof (F : Type -> Type) ts a b : F (typD ts (tvArr a b)) -> F (typD ts a -> typD ts b) :=
+    outof (Iso := @typ2_iso _ _ _ typ_arr F ts a b).
+  Let tvM := @typ1 _ typD _ typ_m.
+  Let m_match := @typ1_match _ typD _ typ_m.
+  Let m_into (F : Type -> Type) ts a : F (m (typD ts a)) -> F (typD ts (tvM a)) :=
+    into (Iso := @typ1_iso _ _ _ typ_m F ts a).
+  Let m_outof (F : Type -> Type) ts a : F (typD ts (tvM a)) -> F (m (typD ts a)) :=
+    outof (Iso := @typ1_iso _ _ _ typ_m F ts a).
+
+  Inductive mexpr : Type :=
+  | Bind : typ -> typ -> mexpr -> mexpr -> mexpr
+  | Ret  : typ -> mexpr -> mexpr
+  | Plus : mexpr -> mexpr -> mexpr
+  | Const : nat -> mexpr
+  | Var : nat -> mexpr
+  | Abs : typ -> mexpr -> mexpr.
+
+  Fixpoint mexprD (g : list typ) (e : mexpr) (t : typ) {struct e} : option (hlist (typD nil) g -> typD nil t).
+  refine (
+      match e with
+        | Var v =>
+          match nth_error g v as nt 
+                return (hlist (typD nil) g -> match nt with
+                                                | None => unit
+                                                | Some t => typD nil t
+                                              end)
+                    -> option (hlist (typD nil) g -> typD nil t)
+          with
+            | None => fun _ => None
+            | Some t' => match typ_cast (fun x => x) nil t' t with
+                           | None => fun _ => None
+                           | Some cast => fun get => Some (fun g => cast (get g))
+                         end
+          end (fun g => hlist_nth g v)
+        | Abs t' body =>
+          arr_match nil (fun ty Ty => option (hlist (typD nil) g -> Ty))
+             (fun d r => 
+                match typ_cast (typD := typD) (fun x => x) nil t' d with 
+                  | None => None
+                  | Some cast_d => 
+                    match mexprD (d :: g) body r with
+                      | None => None
+                      | Some f => Some (fun g x => f (Hcons x g))
+                    end                        
+                end)
+             (fun _ => None)
+             t
+        | Const n =>
+          nat_match nil (fun ty Ty => option (hlist (typD nil) g -> Ty))
+             (fun _ => Some (fun _ => n))
+             (fun _ => None)
+             t
+        | Plus l r =>
+          nat_match nil (fun ty Ty => option (hlist (typD nil) g -> Ty) ->
+                                      option (hlist (typD nil) g -> Ty) ->
+                                      option (hlist (typD nil) g -> Ty))
+             (fun _ l r => 
+                match l , r with
+                  | Some l , Some r => 
+                    Some (fun g => l g + r g)
+                  | _ , _ => None
+                end)
+             (fun _ _ _ => None)
+             t (mexprD g l t) (mexprD g r t)
+        | Ret t' e =>
+          m_match nil (fun ty Ty => option (hlist (typD nil) g -> Ty))
+            (fun t'' => 
+               match typ_cast (fun x => x) nil t' t'' with
+                 | None => None
+                 | Some cast => 
+                   match mexprD g e t' with 
+                     | None => None
+                     | Some r => Some (fun g => ret (cast (r g)))
+                   end
+               end)
+            (fun _ => None)
+            t
+        | Bind t' t'' c k => 
+          m_match nil (fun ty Ty => option (hlist (typD nil) g -> Ty))
+            (fun t''' =>
+               match typ_cast (typD := typD) (fun x => typD nil t' -> m x) nil t'' t''' with
+                 | None => None
+                 | Some cast =>
+                   match mexprD g c (tvM t') , mexprD g k (tvArr t' (tvM t'')) with
+                     | Some cv , Some kv => Some (fun g => bind _ _)
+                     | _ , _ => None
+                   end
+               end)
+            (fun _ => None)
+            t
+      end).
+  (** TODO: Coq doesn't type check when this is inline **)
+  eapply m_outof. eapply cv. eapply g0.
+  eapply cast. eapply m_outof. eapply arr_outof. eapply kv. eapply g0.
+  Defined.
+
+  Definition mexpr_dec (a b : mexpr) : {a = b} + {a <> b}.
+    assert (forall a b : typ, {a = b} + {a <> b}).
+    { admit. }
+    decide equality.
+    decide equality.
+    decide equality.
+  Defined.
+
+  Definition mexpr_eq (a b : mexpr) : option bool :=
+    match mexpr_dec a b with
+      | left _ => Some true
+      | right _ => Some false
+    end.    
+
+  Instance Expr_mexpr : Expr typD mexpr :=
+  { exprD := fun _ g e t => 
+               match Generic.split g with
+                 | existT te env =>
+                   match mexprD te e t with
+                     | None => None
+                     | Some f => Some (f env)
+                   end
+               end
+  ; expr_eq := mexpr_eq
+  }.
+
+  Instance FuncInstance0_plus : FuncInstance0 plus :=
+  { typ0_witness := TypInstance0_app2 typ_arr _ (TypInstance0_app2 typ_arr _ _)
+  ; ctor0 := Abs tvNat (Abs tvNat (Plus (Var 1) (Var 0)))
+  }.
+  simpl.
